<?xml version="1.0" encoding="UTF-8"?>
<!DOCTYPE rdf:RDF [ 
   <!ENTITY proc "http://sweet.jpl.nasa.gov/2.2/procPhysical.owl">    
   <!ENTITY proc2 "http://sweet.jpl.nasa.gov/2.2/procPhysical.owl#">    
   <!ENTITY solu "http://sweet.jpl.nasa.gov/2.2/reprMathSolution.owl">    
   <!ENTITY solu2 "http://sweet.jpl.nasa.gov/2.2/reprMathSolution.owl#">    
   <!ENTITY flui "http://sweet.jpl.nasa.gov/2.2/stateFluid.owl#">    
   <!ENTITY pstate "http://sweet.jpl.nasa.gov/2.2/statePhysical.owl">    
   <!ENTITY owl "http://www.w3.org/2002/07/owl#">    
   <!ENTITY rdf "http://www.w3.org/1999/02/22-rdf-syntax-ns#"> 
   <!ENTITY rdfs "http://www.w3.org/2000/01/rdf-schema#">    
   <!ENTITY xsd "http://www.w3.org/2001/XMLSchema#"> 
]>

<rdf:RDF 
   xml:base = "&flui;"
   xmlns:proc = "&proc;"
   xmlns:proc2 = "&proc2;"
   xmlns:solu = "&solu;"
   xmlns:solu2 = "&solu2;"
   xmlns:flui = "&flui;"
   xmlns:pstate = "&pstate;"
   xmlns:owl = "&owl;"
   xmlns:rdf = "&rdf;"
   xmlns:rdfs = "&rdfs;"
   xmlns:xsd = "&xsd;">

<!-- Ontology Information -->
  <owl:Ontology rdf:about="" owl:versionInfo="1.1">
     <owl:imports rdf:resource="&proc;"/>
     <owl:imports rdf:resource="&solu;"/>
     <owl:imports rdf:resource="&pstate;"/>
  </owl:Ontology>

  <flui:FluidState rdf:about="#Baroclinic">
  </flui:FluidState>

  <flui:FluidState rdf:about="#Barotropic">
    <owl:differentFrom rdf:resource="#Baroclinic" />
  </flui:FluidState>

  <flui:FluidState rdf:about="#Buoyant">
  </flui:FluidState>

  <flui:FluidState rdf:about="#Convective">
  </flui:FluidState>

  <flui:FluidState rdf:about="#Turbulent">
  </flui:FluidState>

  <owl:Class rdf:about="#FluidState">
    <rdfs:subClassOf rdf:resource="&pstate;#PhysicalState"/>
    <rdfs:subClassOf>
      <owl:Restriction>
        <owl:onProperty rdf:resource="&pstate;#hasStateOfMatter" />
        <owl:hasValue rdf:resource="&pstate;#Fluid" />
      </owl:Restriction>
    </rdfs:subClassOf>
  </owl:Class>

  <owl:Class rdf:about="#FluidEquilibriumState">
    <rdfs:subClassOf rdf:resource="#FluidState"/>
    <rdfs:subClassOf rdf:resource="&pstate;#EquilibriumState"/>
  </owl:Class>

  <flui:FluidState rdf:about="#Pressurized"/>

  <flui:FluidState rdf:about="#Unpressurized">
    <owl:differentFrom rdf:resource="#Pressurized"/>
  </flui:FluidState>

  <flui:FluidState rdf:about="#Rareified">
  </flui:FluidState>

  <flui:FluidState rdf:about="#Stratified">
    <owl:sameAs rdf:resource="#Stratification" />
  </flui:FluidState>
  <flui:FluidState rdf:about="#Stratification"/>

  <flui:FluidState rdf:about="#Miscible">
    <rdfs:comment xml:lang="en">Said of two or more liquids that are mutually soluble (i.e. they will dissolve in each other) (McGraw-Hill, 1974).  The chemical property of two or more phases that, when brought together, have the ability to mix and form one phase (after AGI, 1980).</rdfs:comment>
  </flui:FluidState>

  <flui:FluidEquilibriumState rdf:about="#Steric">
  </flui:FluidEquilibriumState>

  <flui:FluidEquilibriumState rdf:about="#Thermosteric">
  </flui:FluidEquilibriumState>

  <flui:FluidEquilibriumState rdf:about="#Halosteric">
  </flui:FluidEquilibriumState>

  <flui:FluidEquilibriumState rdf:about="#SverdrupBalance">
  </flui:FluidEquilibriumState>

  <flui:FluidEquilibriumState rdf:about="#Ekman">
    <rdfs:comment xml:lang="en">Motions describing an equlibrium between pressure gradient force, Coriolis force and the turbulent drag force.</rdfs:comment>
  </flui:FluidEquilibriumState>

  <flui:FluidEquilibriumState rdf:about="#Ageostrophic">
    <owl:differentFrom rdf:resource="#Geostrophic"/>
  </flui:FluidEquilibriumState>

  <flui:FluidEquilibriumState rdf:about="#Geostrophic">
  </flui:FluidEquilibriumState>

  <flui:FluidEquilibriumState rdf:about="#SemiGeostrophic">
  </flui:FluidEquilibriumState>

  <flui:FluidEquilibriumState rdf:about="#QuasiGeostrophic">
    <solu2:approximates rdf:resource="#Geostrophic" />
    <rdfs:comment xml:lang="en">A system or flow that evolves slowly in time compared to the rotation period of the earth, has a length scale of the deformation radius or larger, and undergoes only limited vertical excursions.</rdfs:comment>
  </flui:FluidEquilibriumState>

  <flui:FluidEquilibriumState rdf:about="#Hydrostatic">
  </flui:FluidEquilibriumState>

  <flui:FluidEquilibriumState rdf:about="#QuasiHydrostatic">
    <solu2:approximates rdf:resource="#Hydrostatic" />
  </flui:FluidEquilibriumState>

  <flui:FluidEquilibriumState rdf:about="#Nonhydrostatic">
    <owl:differentFrom rdf:resource="#Hydrostatic"/>
  </flui:FluidEquilibriumState>

</rdf:RDF>
