<?xml version="1.0" encoding="UTF-8"?>

<!DOCTYPE rdf:RDF [

  <!ENTITY root "http://sweet.jpl.nasa.gov/2.1/">
  <!ENTITY rela "&root;reprMathRelation.owl#">
  <!ENTITY mtime "&root;reprTime.owl#">
  <!ENTITY gtime "&root;reprTimeGeologic.owl#">
  <!ENTITY owl "http://www.w3.org/2002/07/owl#">
  <!ENTITY owlt "http://www.w3.org/2006/time#">
  <!ENTITY rdf "http://www.w3.org/1999/02/22-rdf-syntax-ns#">
  <!ENTITY rdfs "http://www.w3.org/2000/01/rdf-schema#">
  <!ENTITY xsd "http://www.w3.org/2001/XMLSchema#">
]>

<rdf:RDF xml:base="&gtime;"
         xmlns:owlt="&owlt;"
         xmlns:gtime="&gtime;"
         xmlns:mtime="&mtime;"
         xmlns:rela="&rela;"
         xmlns:owl="&owl;"
         xmlns:rdf="&rdf;"
         xmlns:rdfs="&rdfs;">

<!-- Ontology Information -->
  <owl:Ontology rdf:about=""
                owl:versionInfo="1.1">
     <owl:imports rdf:resource="&root;reprMathRelation.owl"/>
     <owl:imports rdf:resource="&root;reprTime.owl"/>
  </owl:Ontology>

<!-- Geologic -->
  <owl:Class rdf:about="#Age">
    <rdfs:subClassOf rdf:resource="#GeologicTimeUnit"/>
    <rdfs:subClassOf>
      <owl:Restriction>
        <owl:onProperty rdf:resource="&rela;subsetOf" />
        <owl:someValuesFrom rdf:resource="#Epoch" />
      </owl:Restriction>
    </rdfs:subClassOf>
    <rdfs:comment xml:lang="en">Epochs are divided into ages [millions of years] [Wikipedia]</rdfs:comment>
  </owl:Class>

  <owl:Class rdf:about="#Epoch">
    <rdfs:subClassOf rdf:resource="#GeologicTimeUnit"/>
    <rdfs:subClassOf>
      <owl:Restriction>
        <owl:onProperty rdf:resource="&rela;subsetOf" />
        <owl:someValuesFrom rdf:resource="#Period" />
      </owl:Restriction>
    </rdfs:subClassOf>
    <rdfs:comment xml:lang="en">Periods are divided into epochs [tens of millions of years] [Wikipedia]</rdfs:comment>
  </owl:Class>

  <owl:Class rdf:about="#Period">
    <rdfs:subClassOf rdf:resource="#GeologicTimeUnit"/>
    <rdfs:subClassOf>
      <owl:Restriction>
        <owl:onProperty rdf:resource="&rela;subsetOf" />
        <owl:someValuesFrom rdf:resource="#Era" />
      </owl:Restriction>
    </rdfs:subClassOf>
    <rdfs:comment xml:lang="en">Eras are divided into periods. [Wikipedia]</rdfs:comment>
  </owl:Class>

  <owl:Class rdf:about="#Era">
    <rdfs:subClassOf rdf:resource="#GeologicTimeUnit"/>
    <rdfs:subClassOf>
      <owl:Restriction>
        <owl:onProperty rdf:resource="&rela;subsetOf" />
        <owl:someValuesFrom rdf:resource="#Eon" />
      </owl:Restriction>
    </rdfs:subClassOf>
    <rdfs:comment xml:lang="en">Eons are divided into eras [several hundred million years] [Wikipedia]</rdfs:comment>
  </owl:Class>

  <owl:Class rdf:about="#Eon">
    <rdfs:subClassOf rdf:resource="#GeologicTimeUnit"/>
    <rdfs:subClassOf>
      <owl:Restriction>
        <owl:onProperty rdf:resource="&rela;subsetOf" />
        <owl:someValuesFrom rdf:resource="#Supereon" />
      </owl:Restriction>
    </rdfs:subClassOf>
    <rdfs:comment xml:lang="en">Supereons are divided into eons.  [billions of years] [Wikipedia]</rdfs:comment>
  </owl:Class>

  <owl:Class rdf:about="#Supereon">
    <rdfs:subClassOf rdf:resource="#GeologicTimeUnit"/>
    <rdfs:comment xml:lang="en">The largest defined unit of time is the supereon, composed of eons.] [Wikipedia]</rdfs:comment>
  </owl:Class>

  <owl:Class rdf:about="#GeologicTimeUnit">
    <rdfs:subClassOf rdf:resource="&owlt;ProperInterval"/>
    <rdfs:comment xml:lang="en">The subdivisions of geologic time. The table of geologic time spans are dates and nomenclature defined by the International Commission on Stratigraphy. [Wikipedia]</rdfs:comment>
  </owl:Class>

  <owl:Class rdf:about="#NeotectonicPeriod">
    <rdfs:subClassOf rdf:resource="&mtime;TimeReference"/>
  </owl:Class>

  <owl:Class rdf:about="#IceAge">
    <rdfs:subClassOf rdf:resource="&mtime;TimeReference"/>
  </owl:Class>

  <owl:Class rdf:about="#Interglacial">
    <rdfs:subClassOf rdf:resource="&mtime;TimeReference"/>
    <owl:disjointWith rdf:resource="#IceAge"/>
  </owl:Class>

  <owl:Class rdf:about="#Prehistoric">
    <rdfs:subClassOf rdf:resource="&mtime;TimeReference"/>
  </owl:Class>

</rdf:RDF>
